theories/full_abstraction.v
@@ -1,5 +1,6 @@
 From iris.program_logic Require Import language.
 From cap_machine Require Import simulation linking.
+From cap_machine Require Import addr_reg.
 
 Section Full_Abstraction.
 
@@ -41,3 +42,493 @@ Section Full_Abstraction.
 
 End Full_Abstraction.
 
+From stdpp Require Import base gmap fin_maps list.
+From cap_machine Require Import overlay_cap_lang_sim machine_parameters.
+Ltac inv H := inversion H; clear H; subst.
+
+Section Compile_fully_abstract.
+
+  Variables b_stk e_stk: Addr.
+  Variable stk_pos: (b_stk < e_stk)%a.
+  Context `{MachineParameters}.
+
+  (* Back translating base machine words to overlay words *)
+  Definition backtranslate_word (w: machine_base.Word): base.Word :=
+    match w with
+    | inl n => inl n
+    | inr c => inr (base.Regular c)
+    end.
+
+  (* Trivial back translation from base machine component to overlay component *)
+  Definition decompile (c: cap_lang.machine_component): lang.overlay_component :=
+    match c with
+    | Lib _ _ _ _ (ms, imp, exp) => Lib _ _ _ _ (@fmap (gmap Addr) _ machine_base.Word base.Word backtranslate_word ms, imp, fmap backtranslate_word exp)
+    | Main _ _ _ _ (ms, imp, exp) c_main => Main _ _ _ _ (@fmap (gmap Addr) _ machine_base.Word base.Word backtranslate_word ms, imp, fmap backtranslate_word exp) (backtranslate_word c_main)
+    end.
+
+  Lemma translate_backtranslate_word:
+    forall w,
+      translate_word (backtranslate_word w) = w.
+  Proof. destruct w; reflexivity. Qed.
+
+  Lemma backtranslate_translate_word:
+    forall w,
+      lang.is_global w = true ->
+      backtranslate_word (translate_word w) = w.
+  Proof. intros; destruct w; inv H0; simpl; [|destruct c; try discriminate]; auto. Qed.
+
+  Lemma translate_backtranslate_map K `(EqDecision K) `(Countable K):
+    forall (m: gmap K machine_base.Word),
+      translate_word ∘ backtranslate_word <$> m = m.
+  Proof.
+    intros; eapply map_eq; intros.
+    rewrite lookup_fmap. destruct (m !! i) as [w|] eqn:Hw; simpl; auto.
+    rewrite translate_backtranslate_word; auto.
+  Qed.
+
+  Lemma backtranslate_translate_map K `(EqDecision K) `(Countable K):
+    forall (m: gmap K base.Word),
+    (forall a w, m !! a = Some w -> lang.is_global w = true) ->
+    backtranslate_word ∘ translate_word <$> m = m.
+  Proof.
+    intros; eapply map_eq; intros.
+    rewrite lookup_fmap. destruct (m !! i) as [w|] eqn:Hw; simpl; auto.
+    eapply H1 in Hw. erewrite backtranslate_translate_word; eauto.
+  Qed.
+
+  Lemma compile_decompile:
+    forall comp,
+      compile (decompile comp) = comp.
+  Proof.
+    intros. destruct comp; simpl.
+    - destruct p as [ [ms imp] exp].
+      simpl. rewrite -!map_fmap_compose.
+      rewrite !translate_backtranslate_map //.
+    - destruct p as [ [ms imp] exp].
+      simpl. rewrite -!map_fmap_compose.
+      rewrite !translate_backtranslate_map translate_backtranslate_word //.
+  Qed.
+
+  Lemma decompile_compile:
+    forall comp,
+    well_formed_comp b_stk nat nat_eq_dec nat_countable Word cap_lang.can_address_only cap_lang.pwlW cap_lang.is_global (compile comp) ->
+    decompile (compile comp) = comp.
+  Proof.
+    intros. destruct comp; simpl.
+    - destruct p as [ [ms imp] exp].
+      simpl. inv H0. inv Hwf_pre.
+      rewrite -!map_fmap_compose.
+      rewrite !backtranslate_translate_map; auto.
+      + intros. generalize (Hexp a _ ltac:(rewrite lookup_fmap H0; auto)).
+        intros [A [B C] ]. destruct w; auto.
+        destruct c; simpl in C; try congruence; auto.
+      + intros. generalize (Hnpwl a _ ltac:(rewrite (@lookup_fmap Addr (gmap Addr)) H0 //)).
+        intros [A [B C] ]. destruct w; auto.
+        destruct c; simpl in C; try congruence; auto.
+    - destruct p as [ [ms imp] exp].
+      simpl. inv H0. inv Hwf_pre.
+      rewrite -!map_fmap_compose.
+      rewrite !backtranslate_translate_map; auto.
+      + rewrite backtranslate_translate_word; auto. 
+        destruct Hw_main as [A [B C] ]. destruct w; auto.
+        destruct c; simpl in C; try congruence; auto.
+      + intros. generalize (Hexp a _ ltac:(rewrite lookup_fmap H0; auto)).
+        intros [A [B C] ]. destruct w0; auto.
+        destruct c; simpl in C; try congruence; auto.
+      + intros. generalize (Hnpwl a _ ltac:(rewrite (@lookup_fmap Addr (gmap Addr)) H0 //)).
+        intros [A [B C] ]. destruct w0; auto.
+        destruct c; simpl in C; try congruence; auto.
+  Qed.
+
+  Lemma decompile_preserves_well_formed_comp:
+    forall comp,
+      well_formed_comp b_stk nat nat_eq_dec nat_countable Word cap_lang.can_address_only cap_lang.pwlW cap_lang.is_global comp ->
+      well_formed_comp b_stk nat nat_eq_dec nat_countable base.Word lang.can_address_only lang.pwlW lang.is_global (decompile comp).
+  Proof.
+    destruct comp; intros.
+    - inv H0. inv Hwf_pre.
+      econstructor. econstructor; auto.
+      + intros. rewrite lookup_fmap in H0.
+        erewrite fmap_is_Some in H0.
+        apply Hdisj; auto.
+      + intros. rewrite lookup_fmap in H0.
+        destruct (exp !! s) as [wexp|] eqn:Hwexp; inv H0.
+        eapply Hexp in Hwexp. destruct Hwexp as [A1 [A2 A3] ].
+        destruct wexp; simpl; auto.
+        simpl in A1, A2, A3. destruct c as [ [ [ [p g] b] e] a].
+        rewrite (@dom_fmap_L Addr (gmap Addr) (gset Addr)). auto.
+      + intros. rewrite (@lookup_fmap Addr (gmap Addr)).
+        rewrite fmap_is_Some. eapply Himp; eauto.
+      + intros. rewrite (@lookup_fmap Addr (gmap Addr)) in H0.
+        destruct (ms !! a) as [wexp|] eqn:Hwexp; rewrite Hwexp in H0; inv H0.
+        rewrite (@dom_fmap_L Addr (gmap Addr) (gset Addr)).
+        eapply Hnpwl in Hwexp.
+        destruct wexp; auto.
+      + intros. rewrite (@dom_fmap_L Addr (gmap Addr) (gset Addr)) in H0. auto.
+    - inv H0. inv Hwf_pre.
+      econstructor; simpl.
+      + econstructor; eauto.
+        * intros. rewrite lookup_fmap in H0.
+          erewrite fmap_is_Some in H0.
+          apply Hdisj; auto.
+        * intros. rewrite lookup_fmap in H0.
+          destruct (exp !! s) as [wexp|] eqn:Hwexp; inv H0.
+          eapply Hexp in Hwexp. destruct Hwexp as [A1 [A2 A3] ].
+          destruct wexp; simpl; auto.
+          simpl in A1, A2, A3. destruct c as [ [ [ [p g] b] e] a].
+          rewrite (@dom_fmap_L Addr (gmap Addr) (gset Addr)). auto.
+        * intros. rewrite (@lookup_fmap Addr (gmap Addr)).
+          rewrite fmap_is_Some. eapply Himp; eauto.
+        * intros. rewrite (@lookup_fmap Addr (gmap Addr)) in H0.
+          destruct (ms !! a) as [wexp|] eqn:Hwexp; rewrite Hwexp in H0; inv H0.
+          rewrite (@dom_fmap_L Addr (gmap Addr) (gset Addr)).
+          eapply Hnpwl in Hwexp.
+          destruct wexp; auto.
+        * intros. rewrite (@dom_fmap_L Addr (gmap Addr) (gset Addr)) in H0. auto.
+      + rewrite (@dom_fmap_L Addr (gmap Addr) (gset Addr)). destruct w; auto.
+  Qed.
+
+  Lemma compile_preserves_well_formed_comp:
+    forall comp,
+      well_formed_comp b_stk nat nat_eq_dec nat_countable base.Word lang.can_address_only lang.pwlW lang.is_global comp ->
+      well_formed_comp b_stk nat nat_eq_dec nat_countable Word cap_lang.can_address_only cap_lang.pwlW cap_lang.is_global (compile comp).
+  Proof.
+    destruct comp; intros.
+    - inv H0. inv Hwf_pre.
+      econstructor. econstructor; auto.
+      + intros. rewrite lookup_fmap in H0.
+        erewrite fmap_is_Some in H0.
+        apply Hdisj; auto.
+      + intros. rewrite lookup_fmap in H0.
+        destruct (exp !! s) as [wexp|] eqn:Hwexp; inv H0.
+        eapply Hexp in Hwexp. destruct Hwexp as [A1 [A2 A3] ].
+        destruct wexp; simpl; auto.
+        simpl in A1, A2, A3. destruct c; try congruence.
+        destruct c as [ [ [ [p g] b] e] a].
+        rewrite (@dom_fmap_L Addr (gmap Addr) (gset Addr)). auto.
+      + intros. rewrite (@lookup_fmap Addr (gmap Addr)).
+        rewrite fmap_is_Some. eapply Himp; eauto.
+      + intros. rewrite (@lookup_fmap Addr (gmap Addr)) in H0.
+        destruct (ms !! a) as [wexp|] eqn:Hwexp; rewrite Hwexp in H0; inv H0.
+        rewrite (@dom_fmap_L Addr (gmap Addr) (gset Addr)).
+        eapply Hnpwl in Hwexp. destruct Hwexp as [A [B C] ].
+        destruct wexp; auto.
+        destruct c; simpl in C; try congruence; auto.
+      + intros. rewrite (@dom_fmap_L Addr (gmap Addr) (gset Addr)) in H0. auto.
+    - inv H0. inv Hwf_pre.
+      econstructor; simpl.
+      + econstructor; eauto.
+        * intros. rewrite lookup_fmap in H0.
+          erewrite fmap_is_Some in H0.
+          apply Hdisj; auto.
+        * intros. rewrite lookup_fmap in H0.
+          destruct (exp !! s) as [wexp|] eqn:Hwexp; inv H0.
+          eapply Hexp in Hwexp. destruct Hwexp as [A1 [A2 A3] ].
+          destruct wexp; simpl; auto.
+          simpl in A1, A2, A3. destruct c; try congruence.
+          destruct c as [ [ [ [p g] b] e] a].
+          rewrite (@dom_fmap_L Addr (gmap Addr) (gset Addr)). auto.
+        * intros. rewrite (@lookup_fmap Addr (gmap Addr)).
+          rewrite fmap_is_Some. eapply Himp; eauto.
+        * intros. rewrite (@lookup_fmap Addr (gmap Addr)) in H0.
+          destruct (ms !! a) as [wexp|] eqn:Hwexp; rewrite Hwexp in H0; inv H0.
+          rewrite (@dom_fmap_L Addr (gmap Addr) (gset Addr)).
+          eapply Hnpwl in Hwexp. destruct Hwexp as [A [B C] ].
+          destruct wexp; auto.
+          destruct c; simpl in C; try congruence; auto.
+        * intros. rewrite (@dom_fmap_L Addr (gmap Addr) (gset Addr)) in H0. auto.
+      + rewrite (@dom_fmap_L Addr (gmap Addr) (gset Addr)). destruct w; auto.
+        destruct Hw_main as [A [B C] ].
+        destruct c; simpl in C; try congruence; auto.
+  Qed.
+
+  Lemma map_fmap_union {K A B} `{EqDecision K} `{Countable K} (f : A → B) (m1 m2 : gmap K A) :
+    f <$> (map_union m1 m2) = map_union (f <$> m1) (f <$> m2).
+  Proof.
+    apply map_eq; intros i. apply option_eq; intros x.
+    rewrite lookup_fmap !lookup_union !lookup_fmap.
+    destruct (m1 !! i), (m2 !! i); auto.
+  Qed.
+
+  (* I hate Coq *)
+  Lemma backtranslate_resolve_imports:
+    forall imp exp ms
+      (Himpdisj: forall s1 s2 a, (s1, a) ∈ imp -> (s2, a) ∈ imp -> s1 = s2),
+      @gmap_fmap Addr _ _ Word base.Word backtranslate_word (resolve_imports nat nat_eq_dec nat_countable Word imp exp ms) =
+      resolve_imports nat nat_eq_dec nat_countable base.Word imp (backtranslate_word <$> exp) (@gmap_fmap Addr _ _ Word base.Word backtranslate_word ms).
+  Proof.
+  intros. apply map_eq.
+  intros a.
+  assert (Hx: forall x, (exists s, (s, x) ∈ imp) \/ ~ (exists s, (s, x) ∈ imp)).
+  { intros.
+    generalize (@set_Exists_dec (nat * Addr) (imports nat nat_eq_dec nat_countable) ltac:(apply _) ltac:(apply _) ltac:(apply _) ltac:(apply _) ltac:(apply _) ltac:(apply _) ltac:(apply _) ltac:(apply _) ltac:(apply _) (fun s => s.2 = x) ltac:(intros s; destruct (addr_eq_dec s.2 x); [left; auto|right; auto]) imp).
+    destruct 1.
+    - destruct s. destruct x0. destruct H0. simpl in H1. inv H1.
+      left; exists n; auto.
+    - right. red; intros. destruct H0.
+      eapply n. exists (x0, x). split; auto. }
+  destruct (Hx a).
+  - destruct H0 as [s Hin].
+    destruct (resolve_imports_spec_in nat nat_eq_dec nat_countable Word imp exp ms a s Himpdisj Hin) as [ [A1 A2] | [wexp [A1 A2] ] ].
+    + destruct (resolve_imports_spec_in nat nat_eq_dec nat_countable base.Word imp (backtranslate_word <$> exp) (@gmap_fmap Addr _ _ Word base.Word backtranslate_word ms) a s Himpdisj Hin) as [ [B1 B2] | [wexp [B1 B2] ] ].
+      * rewrite B2. rewrite lookup_fmap A2. rewrite (@lookup_fmap Addr (gmap Addr) _ _ _ _ _ _ _ _ _ _ _ backtranslate_word ms a). reflexivity.
+      * rewrite lookup_fmap in B1. rewrite A1 in B1; inv B1.
+    + destruct (resolve_imports_spec_in nat nat_eq_dec nat_countable base.Word imp (backtranslate_word <$> exp) (@gmap_fmap Addr _ _ Word base.Word backtranslate_word ms) a s Himpdisj Hin) as [ [B1 B2] | [wexp' [B1 B2] ] ].
+      * rewrite lookup_fmap A1 in B1; inv B1.
+      * rewrite lookup_fmap A1 in B1; inv B1.
+        rewrite B2. rewrite lookup_fmap A2. reflexivity.
+  - erewrite resolve_imports_spec_not_in; eauto.
+    rewrite lookup_fmap. erewrite resolve_imports_spec_not_in; eauto.
+    rewrite (@lookup_fmap Addr (gmap Addr) _ _ _ _ _ _ _ _ _ _ _ backtranslate_word ms a). reflexivity.
+  Qed.
+
+  Lemma translate_resolve_imports:
+    forall imp exp ms
+      (Himpdisj: forall s1 s2 a, (s1, a) ∈ imp -> (s2, a) ∈ imp -> s1 = s2),
+      @gmap_fmap Addr _ _ base.Word Word translate_word (resolve_imports nat nat_eq_dec nat_countable base.Word imp exp ms) =
+      resolve_imports nat nat_eq_dec nat_countable Word imp (translate_word <$> exp) (@gmap_fmap Addr _ _ base.Word Word translate_word ms).
+  Proof.
+  intros. apply map_eq.
+  intros a.
+  assert (Hx: forall x, (exists s, (s, x) ∈ imp) \/ ~ (exists s, (s, x) ∈ imp)).
+  { intros.
+    generalize (@set_Exists_dec (nat * Addr) (imports nat nat_eq_dec nat_countable) ltac:(apply _) ltac:(apply _) ltac:(apply _) ltac:(apply _) ltac:(apply _) ltac:(apply _) ltac:(apply _) ltac:(apply _) ltac:(apply _) (fun s => s.2 = x) ltac:(intros s; destruct (addr_eq_dec s.2 x); [left; auto|right; auto]) imp).
+    destruct 1.
+    - destruct s. destruct x0. destruct H0. simpl in H1. inv H1.
+      left; exists n; auto.
+    - right. red; intros. destruct H0.
+      eapply n. exists (x0, x). split; auto. }
+  destruct (Hx a).
+  - destruct H0 as [s Hin].
+    destruct (resolve_imports_spec_in nat nat_eq_dec nat_countable base.Word imp exp ms a s Himpdisj Hin) as [ [A1 A2] | [wexp [A1 A2] ] ].
+    + destruct (resolve_imports_spec_in nat nat_eq_dec nat_countable Word imp (translate_word <$> exp) (@gmap_fmap Addr _ _ base.Word Word translate_word ms) a s Himpdisj Hin) as [ [B1 B2] | [wexp [B1 B2] ] ].
+      * rewrite B2. rewrite lookup_fmap A2. rewrite (@lookup_fmap Addr (gmap Addr) _ _ _ _ _ _ _ _ _ _ _ translate_word ms a). reflexivity.
+      * rewrite lookup_fmap in B1. rewrite A1 in B1; inv B1.
+    + destruct (resolve_imports_spec_in nat nat_eq_dec nat_countable Word imp (translate_word <$> exp) (@gmap_fmap Addr _ _ base.Word Word translate_word ms) a s Himpdisj Hin) as [ [B1 B2] | [wexp' [B1 B2] ] ].
+      * rewrite lookup_fmap A1 in B1; inv B1.
+      * rewrite lookup_fmap A1 in B1; inv B1.
+        rewrite B2. rewrite lookup_fmap A2. reflexivity.
+  - erewrite resolve_imports_spec_not_in; eauto.
+    rewrite lookup_fmap. erewrite resolve_imports_spec_not_in; eauto.
+    rewrite (@lookup_fmap Addr (gmap Addr) _ _ _ _ _ _ _ _ _ _ _ translate_word ms a). reflexivity.
+  Qed.
+
+  Lemma decompile_preserves_link:
+    forall context comp prog,
+      link b_stk nat nat_eq_dec nat_countable Word cap_lang.can_address_only cap_lang.pwlW cap_lang.is_global context comp prog ->
+      link b_stk nat nat_eq_dec nat_countable base.Word lang.can_address_only lang.pwlW lang.is_global (decompile context) (decompile comp) (decompile prog).
+  Proof.
+    intros. inv H0; simpl decompile.
+    - destruct comp1 as [ [ms1 imp1] exp1].
+      destruct comp2 as [ [ms2 imp2] exp2].
+      destruct comp0 as [ [m2 imp] exp].
+      econstructor; [|eapply decompile_preserves_well_formed_comp in Hwf_l; simpl; eapply Hwf_l|eapply decompile_preserves_well_formed_comp in Hwf_r; simpl; eapply Hwf_r].
+      inv Hlink. econstructor.
+      + intros. rewrite lookup_fmap in H0.
+        erewrite fmap_is_Some in H0.
+        rewrite lookup_fmap in H1.
+        erewrite fmap_is_Some in H1.
+        eapply Hms_disj; eauto.
+      + apply map_eq. intros.
+        erewrite lookup_merge; [|reflexivity].
+        rewrite !lookup_fmap.
+        erewrite lookup_merge; [|reflexivity].
+        destruct (exp1 !! i) as [w1|] eqn:Hw1; rewrite Hw1 /= //.
+      + intros. split; intros.
+        * eapply Himp in H0. destruct H0. split; auto.
+          rewrite lookup_fmap. rewrite H1. auto.
+        * destruct H0. rewrite lookup_fmap in H1.
+          eapply Himp. split; auto.
+          match goal with |- ?X = None => destruct X; simpl in H1; auto; inv H1 end.
+      + match goal with |- backtranslate_word <$> resolve_imports nat nat_eq_dec nat_countable Word imp2 ?exp ?ms = _ => generalize (backtranslate_resolve_imports imp2 exp ms ltac:(inv Hwf_r; inv Hwf_pre; auto)) end.
+        intro X. etransitivity; [apply X|].
+        f_equal. rewrite -map_fmap_union.
+        apply backtranslate_resolve_imports. inv Hwf_l. inv Hwf_pre; auto.
+    - destruct comp1 as [ [ms1 imp1] exp1].
+      destruct comp2 as [ [ms2 imp2] exp2].
+      destruct comp0 as [ [m2 imp] exp].
+      econstructor; [|eapply decompile_preserves_well_formed_comp in Hwf_l; simpl; eapply Hwf_l|eapply decompile_preserves_well_formed_comp in Hwf_r; simpl; eapply Hwf_r].
+      inv Hlink. econstructor.
+      + intros. rewrite lookup_fmap in H0.
+        erewrite fmap_is_Some in H0.
+        rewrite lookup_fmap in H1.
+        erewrite fmap_is_Some in H1.
+        eapply Hms_disj; eauto.
+      + apply map_eq. intros.
+        erewrite lookup_merge; [|reflexivity].
+        rewrite !lookup_fmap.
+        erewrite lookup_merge; [|reflexivity].
+        destruct (exp1 !! i) as [w1|] eqn:Hw1; rewrite Hw1 /= //.
+      + intros. split; intros.
+        * eapply Himp in H0. destruct H0. split; auto.
+          rewrite lookup_fmap. rewrite H1. auto.
+        * destruct H0. rewrite lookup_fmap in H1.
+          eapply Himp. split; auto.
+          match goal with |- ?X = None => destruct X; simpl in H1; auto; inv H1 end.
+      + match goal with |- backtranslate_word <$> resolve_imports nat nat_eq_dec nat_countable Word imp2 ?exp ?ms = _ => generalize (backtranslate_resolve_imports imp2 exp ms ltac:(inv Hwf_r; inv Hwf_pre; auto)) end.
+        intro X. etransitivity; [apply X|].
+        f_equal. rewrite -map_fmap_union.
+        apply backtranslate_resolve_imports. inv Hwf_l. inv Hwf_pre; auto.
+    - destruct comp1 as [ [ms1 imp1] exp1].
+      destruct comp2 as [ [ms2 imp2] exp2].
+      destruct comp0 as [ [m2 imp] exp].
+      econstructor; [|eapply decompile_preserves_well_formed_comp in Hwf_l; simpl; eapply Hwf_l|eapply decompile_preserves_well_formed_comp in Hwf_r; simpl; eapply Hwf_r].
+      inv Hlink. econstructor.
+      + intros. rewrite lookup_fmap in H0.
+        erewrite fmap_is_Some in H0.
+        rewrite lookup_fmap in H1.
+        erewrite fmap_is_Some in H1.
+        eapply Hms_disj; eauto.
+      + apply map_eq. intros.
+        erewrite lookup_merge; [|reflexivity].
+        rewrite !lookup_fmap.
+        erewrite lookup_merge; [|reflexivity].
+        destruct (exp1 !! i) as [w1|] eqn:Hw1; rewrite Hw1 /= //.
+      + intros. split; intros.
+        * eapply Himp in H0. destruct H0. split; auto.
+          rewrite lookup_fmap. rewrite H1. auto.
+        * destruct H0. rewrite lookup_fmap in H1.
+          eapply Himp. split; auto.
+          match goal with |- ?X = None => destruct X; simpl in H1; auto; inv H1 end.
+      + match goal with |- backtranslate_word <$> resolve_imports nat nat_eq_dec nat_countable Word imp2 ?exp ?ms = _ => generalize (backtranslate_resolve_imports imp2 exp ms ltac:(inv Hwf_r; inv Hwf_pre; auto)) end.
+        intro X. etransitivity; [apply X|].
+        f_equal. rewrite -map_fmap_union.
+        apply backtranslate_resolve_imports. inv Hwf_l. inv Hwf_pre; auto.
+  Qed.
+
+  Lemma compile_preserves_link:
+    forall context comp prog,
+      link b_stk nat nat_eq_dec nat_countable base.Word lang.can_address_only lang.pwlW lang.is_global context comp prog ->
+      link b_stk nat nat_eq_dec nat_countable Word cap_lang.can_address_only cap_lang.pwlW cap_lang.is_global (compile context) (compile comp) (compile prog).
+  Proof.
+    intros. inv H0; simpl compile.
+    - destruct comp1 as [ [ms1 imp1] exp1].
+      destruct comp2 as [ [ms2 imp2] exp2].
+      destruct comp0 as [ [m2 imp] exp].
+      econstructor; [|eapply compile_preserves_well_formed_comp in Hwf_l; simpl; eapply Hwf_l|eapply compile_preserves_well_formed_comp in Hwf_r; simpl; eapply Hwf_r].
+      inv Hlink. econstructor.
+      + intros. rewrite lookup_fmap in H0.
+        erewrite fmap_is_Some in H0.
+        rewrite lookup_fmap in H1.
+        erewrite fmap_is_Some in H1.
+        eapply Hms_disj; eauto.
+      + apply map_eq. intros.
+        erewrite lookup_merge; [|reflexivity].
+        rewrite !lookup_fmap.
+        erewrite lookup_merge; [|reflexivity].
+        destruct (exp1 !! i) as [w1|] eqn:Hw1; rewrite Hw1 /= //.
+      + intros. split; intros.
+        * eapply Himp in H0. destruct H0. split; auto.
+          rewrite lookup_fmap. rewrite H1. auto.
+        * destruct H0. rewrite lookup_fmap in H1.
+          eapply Himp. split; auto.
+          match goal with |- ?X = None => destruct X; simpl in H1; auto; inv H1 end.
+      + match goal with |- translate_word <$> resolve_imports nat nat_eq_dec nat_countable base.Word imp2 ?exp ?ms = _ => generalize (translate_resolve_imports imp2 exp ms ltac:(inv Hwf_r; inv Hwf_pre; auto)) end.
+        intro X. etransitivity; [apply X|].
+        f_equal. rewrite -map_fmap_union.
+        apply translate_resolve_imports. inv Hwf_l. inv Hwf_pre; auto.
+    - destruct comp1 as [ [ms1 imp1] exp1].
+      destruct comp2 as [ [ms2 imp2] exp2].
+      destruct comp0 as [ [m2 imp] exp].
+      econstructor; [|eapply compile_preserves_well_formed_comp in Hwf_l; simpl; eapply Hwf_l|eapply compile_preserves_well_formed_comp in Hwf_r; simpl; eapply Hwf_r].
+      inv Hlink. econstructor.
+      + intros. rewrite lookup_fmap in H0.
+        erewrite fmap_is_Some in H0.
+        rewrite lookup_fmap in H1.
+        erewrite fmap_is_Some in H1.
+        eapply Hms_disj; eauto.
+      + apply map_eq. intros.
+        erewrite lookup_merge; [|reflexivity].
+        rewrite !lookup_fmap.
+        erewrite lookup_merge; [|reflexivity].
+        destruct (exp1 !! i) as [w1|] eqn:Hw1; rewrite Hw1 /= //.
+      + intros. split; intros.
+        * eapply Himp in H0. destruct H0. split; auto.
+          rewrite lookup_fmap. rewrite H1. auto.
+        * destruct H0. rewrite lookup_fmap in H1.
+          eapply Himp. split; auto.
+          match goal with |- ?X = None => destruct X; simpl in H1; auto; inv H1 end.
+      + match goal with |- translate_word <$> resolve_imports nat nat_eq_dec nat_countable base.Word imp2 ?exp ?ms = _ => generalize (translate_resolve_imports imp2 exp ms ltac:(inv Hwf_r; inv Hwf_pre; auto)) end.
+        intro X. etransitivity; [apply X|].
+        f_equal. rewrite -map_fmap_union.
+        apply translate_resolve_imports. inv Hwf_l. inv Hwf_pre; auto.
+    - destruct comp1 as [ [ms1 imp1] exp1].
+      destruct comp2 as [ [ms2 imp2] exp2].
+      destruct comp0 as [ [m2 imp] exp].
+      econstructor; [|eapply compile_preserves_well_formed_comp in Hwf_l; simpl; eapply Hwf_l|eapply compile_preserves_well_formed_comp in Hwf_r; simpl; eapply Hwf_r].
+      inv Hlink. econstructor.
+      + intros. rewrite lookup_fmap in H0.
+        erewrite fmap_is_Some in H0.
+        rewrite lookup_fmap in H1.
+        erewrite fmap_is_Some in H1.
+        eapply Hms_disj; eauto.
+      + apply map_eq. intros.
+        erewrite lookup_merge; [|reflexivity].
+        rewrite !lookup_fmap.
+        erewrite lookup_merge; [|reflexivity].
+        destruct (exp1 !! i) as [w1|] eqn:Hw1; rewrite Hw1 /= //.
+      + intros. split; intros.
+        * eapply Himp in H0. destruct H0. split; auto.
+          rewrite lookup_fmap. rewrite H1. auto.
+        * destruct H0. rewrite lookup_fmap in H1.
+          eapply Himp. split; auto.
+          match goal with |- ?X = None => destruct X; simpl in H1; auto; inv H1 end.
+      + match goal with |- translate_word <$> resolve_imports nat nat_eq_dec nat_countable base.Word imp2 ?exp ?ms = _ => generalize (translate_resolve_imports imp2 exp ms ltac:(inv Hwf_r; inv Hwf_pre; auto)) end.
+        intro X. etransitivity; [apply X|].
+        f_equal. rewrite -map_fmap_union.
+        apply translate_resolve_imports. inv Hwf_l. inv Hwf_pre; auto.
+  Qed.
+
+  Lemma decompile_preserves_is_context:
+    forall context comp prog,
+      is_context b_stk nat nat_eq_dec nat_countable Word cap_lang.can_address_only cap_lang.pwlW cap_lang.is_global context comp prog ->
+      is_context b_stk nat nat_eq_dec nat_countable base.Word lang.can_address_only lang.pwlW lang.is_global (decompile context) (decompile comp) (decompile prog).
+  Proof.
+    intros. inv H0. econstructor.
+    destruct His_program as [Hlink His_program].
+    split; [eapply decompile_preserves_link; eauto|].
+    inv His_program. simpl. econstructor; auto.
+    eapply decompile_preserves_well_formed_comp in Hwfcomp.
+    apply Hwfcomp.
+  Qed.
+
+  Lemma compile_preserves_is_context:
+    forall context comp prog,
+      is_context b_stk nat nat_eq_dec nat_countable base.Word lang.can_address_only lang.pwlW lang.is_global context comp prog ->
+      is_context b_stk nat nat_eq_dec nat_countable Word cap_lang.can_address_only cap_lang.pwlW cap_lang.is_global (compile context) (compile comp) (compile prog).
+  Proof.
+    intros. inv H0. econstructor.
+    destruct His_program as [Hlink His_program].
+    split; [eapply compile_preserves_link; eauto|].
+    inv His_program. simpl. econstructor; auto.
+    eapply compile_preserves_well_formed_comp in Hwfcomp.
+    apply Hwfcomp.
+  Qed.
+
+  (* Definition of fully abstract specialized for the overlay and base capability machine semantics *)
+  Definition fully_abstract := is_fully_abstract lang.overlay_lang cap_lang.cap_lang b_stk nat _ _ base.Word machine_base.Word lang.can_address_only lang.pwlW lang.is_global cap_lang.can_address_only cap_lang.pwlW cap_lang.is_global (lang.initial_state b_stk e_stk) (cap_lang.initial_state call.r_stk b_stk e_stk).
+
+  Theorem compile_fully_abstract:
+    fully_abstract compile.
+  Proof.
+    intros compS1 compS2; split; intros.
+    - red; intros. generalize (decompile_preserves_is_context _ _ _ H1).
+      rewrite decompile_compile; [|inv H1; destruct His_program as [A B]; inv A; auto].
+      intro Hcontext1.
+      generalize (decompile_preserves_is_context _ _ _ H2).
+      rewrite decompile_compile; [|inv H2; destruct His_program as [A B]; inv A; auto].
+      intro Hcontext2.
+      generalize (H0 _ _ _ Hcontext1 Hcontext2). intros X.
+      split; intros.
+      + destruct H3 as [s1 [step1 Hfinal1] ].
+        deterministic
+        generalize (fsim_backwards lang.overlay_lang cap_lang.cap_lang cap_lang.cap_lang_determ).
+      generalize fsim_terminates.
+      generalize (@overlay_to_cap_lang_fsim b_stk e_stk stk_pos H).
+
+
+
+
+
+
+End Compile_fully_abstract.
