theories/linking.v
@@ -33,7 +33,7 @@ Section Linking.
         (Hdisj: forall s, is_Some (exp !! s) -> ~ exists a, (s, a) ∈ imp)
         (Hexp: forall s w, exp !! s = Some w -> can_address_only w (dom _ ms) /\ pwl w = false /\ is_global w = true)
         (Himp: forall s a, (s, a) ∈ imp -> is_Some (ms !! a))
-        (Himpdisj: forall s1 a1 s2 a2, (s1, a2) ∈ imp -> (s2, a2) ∈ imp -> s1 = s2 \/ a1 <> a2)
+        (Himpdisj: forall s1 s2 a, (s1, a) ∈ imp -> (s2, a) ∈ imp -> s1 = s2)
         (Hnpwl: forall a w, ms !! a = Some w -> can_address_only w (dom _ ms) /\ pwl w = false /\ is_global w = true)
         (Hdisjstk: forall a, a ∈ dom (gset _) ms -> (e_stk <= a)%a), (* \/ (a < b_stk)%a *)
         well_formed_pre_comp (ms, imp, exp).
@@ -61,52 +61,53 @@ Section Linking.
 
   Lemma resolve_imports_spec:
     forall imp exp ms a
-      (Himpdisj: forall s1 a1 s2 a2, (s1, a2) ∈ imp -> (s2, a2) ∈ imp -> s1 = s2 \/ a1 <> a2),
+      (Himpdisj: forall s1 s2 a, (s1, a) ∈ imp -> (s2, a) ∈ imp -> s1 = s2),
       ((~ exists s, (s, a) ∈ imp) ->
        (resolve_imports imp exp ms) !! a = ms !! a) /\
       (forall s, (s, a) ∈ imp ->
        (exp !! s = None /\ (resolve_imports imp exp ms) !! a = ms !! a) \/ (exists wexp, exp !! s = Some wexp /\ (resolve_imports imp exp ms) !! a = Some wexp)).
   Proof.
-    intros imp exp ms a. eapply (set_fold_ind_L (fun m imp => (forall s1 a1 s2 a2, (s1, a2) ∈ imp -> (s2, a2) ∈ imp -> s1 = s2 \/ a1 <> a2) -> ((~ exists s, (s, a) ∈ imp) -> m !! a = ms !! a) /\ (forall s, (s, a) ∈ imp -> (exp !! s = None /\ m !! a = ms !! a) \/ (exists wexp, exp !! s = Some wexp /\ m !! a = Some wexp))) (fun '(s, a) m => match exp !! s with Some w => <[a:=w]> m | None => m end)); eauto.
+    intros imp exp ms a. eapply (set_fold_ind_L (fun m imp => (forall s1 s2 a, (s1, a) ∈ imp -> (s2, a) ∈ imp -> s1 = s2) -> ((~ exists s, (s, a) ∈ imp) -> m !! a = ms !! a) /\ (forall s, (s, a) ∈ imp -> (exp !! s = None /\ m !! a = ms !! a) \/ (exists wexp, exp !! s = Some wexp /\ m !! a = Some wexp))) (fun '(s, a) m => match exp !! s with Some w => <[a:=w]> m | None => m end)); eauto.
     { intros. split; auto. intros.
       eapply elem_of_empty in H0; elim H0; auto. }
     intros. destruct x. split.
     { intros. destruct (exp !! s).
       - rewrite lookup_insert_ne; auto.
         + apply H0.
-          * intros. eapply H1; eapply elem_of_union; right; auto.
+          * intros. eapply H1; eapply elem_of_union; right; eauto.
           * intro Y. destruct Y as [sy Hiny].
-            eapply H2. exists sy. eapply elem_of_union. right; auto.
+            eapply H2. exists sy. eapply elem_of_union. right; eauto.
         + intro; subst a0. eapply H2. exists s.
-          eapply elem_of_union. left.  eapply elem_of_singleton. reflexivity.
-      - apply H0. 
-        + intros. eapply H1; eapply elem_of_union; right; auto.
+          eapply elem_of_union. left. eapply elem_of_singleton. reflexivity.
+      - apply H0.
+        + intros. eapply H1; eapply elem_of_union; right; eauto.
         + intro Y. destruct Y as [sy Hiny].
           eapply H2. exists sy. eapply elem_of_union. right; auto. }
     { intros; destruct (exp !! s) eqn:Hexp.
       - destruct (addr_eq_dec a0 a).
         + subst a0; rewrite lookup_insert.
           right. assert (s0 = s) as ->; eauto.
-          generalize (H1 s a s0 a ltac:(eapply elem_of_union_l; eapply elem_of_singleton; eauto) H2).
-          intros [Z | Z]; [auto|elim Z; auto].
+          eapply elem_of_union in H2. destruct H2.
+          * generalize (proj1 (elem_of_singleton _ _) H2). inversion 1; subst; auto.
+          * eapply (H1 s0 s a); [eapply elem_of_union_r; auto|eapply elem_of_union_l; eapply elem_of_singleton; eauto].
         + rewrite lookup_insert_ne; auto.
           eapply elem_of_union in H2; destruct H2.
           * erewrite elem_of_singleton in H2. inversion H2; congruence.
           * eapply H0; auto.
-            intros; apply H1; eapply elem_of_union; right; auto.
+            intros; eapply H1; eapply elem_of_union; right; eauto.
       - eapply elem_of_union in H2. destruct H2.
         + erewrite elem_of_singleton in H2. inversion H2; subst; clear H2.
-          left; split; auto. apply (proj1 (H0 ltac:(intros; eapply H1; eapply elem_of_union; right; auto))).
+          left; split; auto. eapply (proj1 (H0 ltac:(intros; eapply H1; eapply elem_of_union; right; eauto))).
           intro Y. destruct Y as [sy Hsy].
-          generalize (H1 s a0 sy a0 ltac:(eapply elem_of_union_l; eapply elem_of_singleton; eauto) ltac:(eapply elem_of_union_r; auto)).
-          intros [Z|Z]; [subst; elim H; auto|elim Z; auto].
+          eapply H. replace s with sy; auto.
+          eapply H1; [eapply elem_of_union_r; eauto| eapply elem_of_union_l; eapply elem_of_singleton; eauto].
         + eapply H0; auto.
-          intros; eapply H1; eapply elem_of_union_r; auto. }
+          intros; eapply H1; eapply elem_of_union_r; eauto. }
   Qed.
 
   Lemma resolve_imports_spec_in:
     forall imp exp ms a s
-      (Himpdisj: forall s1 a1 s2 a2, (s1, a2) ∈ imp -> (s2, a2) ∈ imp -> s1 = s2 \/ a1 <> a2),
+      (Himpdisj: forall s1 s2 a, (s1, a) ∈ imp -> (s2, a) ∈ imp -> s1 = s2),
       (s, a) ∈ imp ->
       (exp !! s = None /\ (resolve_imports imp exp ms) !! a = ms !! a) \/ (exists wexp, exp !! s = Some wexp /\ (resolve_imports imp exp ms) !! a = Some wexp).
   Proof.
@@ -115,7 +116,7 @@ Section Linking.
 
   Lemma resolve_imports_spec_not_in:
     forall imp exp ms a
-      (Himpdisj: forall s1 a1 s2 a2, (s1, a2) ∈ imp -> (s2, a2) ∈ imp -> s1 = s2 \/ a1 <> a2),
+      (Himpdisj: forall s1 s2 a, (s1, a) ∈ imp -> (s2, a) ∈ imp -> s1 = s2),
       ((~ exists s, (s, a) ∈ imp) ->
        (resolve_imports imp exp ms) !! a = ms !! a).
   Proof.
